Makefile
@@ -21,9 +21,9 @@ else
 ARCHDIRS=$(ARCH)_$(BITSIZE) $(ARCH)
 endif
 
-DIRS=lib common $(ARCHDIRS) backend cfrontend driver \
+DIRS=lib common $(ARCHDIRS) backend cfrontend driver debug\
   flocq/Core flocq/Prop flocq/Calc flocq/Appli exportclight \
-  cparser cparser/MenhirLib cklr
+  cparser cparser/validator cklr
 
 RECDIRS=lib common $(ARCHDIRS) backend cfrontend driver flocq exportclight \
   cparser cklr
@@ -67,7 +67,7 @@ VLIB=Axioms.v Coqlib.v Intv.v Maps.v Heaps.v Lattice.v Ordered.v \
 COMMON=Errors.v AST.v Linking.v \
   Events.v Globalenvs.v Memdata.v Memtype.v Memory.v BlockNames.v \
   Values.v Smallstep.v Behaviors.v Switch.v Determinism.v Unityping.v \
-  LanguageInterface.v Invariant.v CallconvAlgebra.v ModuleSemantics.v \
+  LanguageInterface.v Invariant.v CallconvAlgebra.v \
   Separation.v \
   CKLR.v Valuesrel.v Eventsrel.v Globalenvsrel.v \
 
@@ -114,7 +114,7 @@ BACKEND=\
 CFRONTEND=Ctypes.v Cop.v Csyntax.v Csem.v Ctyping.v Cstrategy.v Cexec.v \
   Initializers.v Initializersproof.v \
   SimplExpr.v SimplExprspec.v SimplExprproof.v \
-  Clight.v ClightBigstep.v ClightLink.v SimplLocals.v SimplLocalsproof.v \
+  Clight.v ClightBigstep.v SimplLocals.v SimplLocalsproof.v \
   Cshmgen.v Cshmgenproof.v \
   Csharpminor.v Cminorgen.v Cminorgenproof.v \
   Coprel.v Clightrel.v \
@@ -161,7 +161,7 @@ endif
 proof: $(FILES:.v=.vo)
 
 # Turn off some warnings for compiling Flocq
-flocq/%.vo: COQCOPTS+=-w -compatibility-notation
+flocq/%.vo: COQCOPTS+=-w -deprecated-implicit-arguments
 
 extraction: extraction/STAMP
 
@@ -190,11 +190,18 @@ FORCE:
 
 .PHONY: proof extraction runtime FORCE
 
-documentation: $(FILES)
+documentation: doc/coq2html $(FILES)
 	mkdir -p doc/html
 	rm -f doc/html/*.html
-	coq2html -d doc/html/ -base compcert -short-names doc/*.glob \
+	doc/coq2html -o 'doc/html/%.html' doc/*.glob \
           $(filter-out doc/coq2html cparser/Parser.v, $^)
+	cp doc/coq2html.css doc/coq2html.js doc/html/
+
+doc/coq2html: doc/coq2html.ml
+	ocamlopt -w +a-29 -o doc/coq2html str.cmxa doc/coq2html.ml
+
+doc/coq2html.ml: doc/coq2html.mll
+	ocamllex -q doc/coq2html.mll
 
 tools/ndfun: tools/ndfun.ml
 	ocamlopt -o tools/ndfun str.cmxa tools/ndfun.ml
@@ -231,6 +238,8 @@ compcert.ini: Makefile.config
          echo "has_runtime_lib=$(HAS_RUNTIME_LIB)"; \
          echo "has_standard_headers=$(HAS_STANDARD_HEADERS)"; \
          echo "asm_supports_cfi=$(ASM_SUPPORTS_CFI)"; \
+         echo "struct_passing_style=$(STRUCT_PASSING)"; \
+         echo "struct_return_style=$(STRUCT_RETURN)"; \
 	 echo "response_file_style=$(RESPONSEFILE)";) \
         > compcert.ini
 
@@ -240,9 +249,7 @@ driver/Version.ml: VERSION
 	>driver/Version.ml
 
 cparser/Parser.v: cparser/Parser.vy
-	@rm -f $@
-	$(MENHIR) $(MENHIR_FLAGS) --coq cparser/Parser.vy
-	@chmod a-w $@
+	$(MENHIR) --coq cparser/Parser.vy
 
 depend: $(GENERATED) depend1
 
@@ -261,27 +268,17 @@ install:
 ifeq ($(CLIGHTGEN),true)
 	install -m 0755 ./clightgen $(BINDIR)
 endif
-ifeq ($(INSTALL_COQDEV),true)
-	install -d $(COQDEVDIR)
-	for d in $(DIRS); do \
-          install -d $(COQDEVDIR)/$$d && \
-          install -m 0644 $$d/*.vo $(COQDEVDIR)/$$d/; \
-	done
-	install -m 0644 ./VERSION $(COQDEVDIR)
-	@(echo "To use, pass the following to coq_makefile or add the following to _CoqProject:"; echo "-R $(COQDEVDIR) compcert") > $(COQDEVDIR)/README
-endif
-
 
 clean:
 	rm -f $(patsubst %, %/*.vo, $(DIRS))
 	rm -f $(patsubst %, %/.*.aux, $(DIRS))
 	rm -rf doc/html doc/*.glob
+	rm -f doc/coq2html.ml doc/coq2html doc/*.cm? doc/*.o
 	rm -f driver/Version.ml
 	rm -f compcert.ini
 	rm -f extraction/STAMP extraction/*.ml extraction/*.mli .depend.extr
 	rm -f tools/ndfun tools/modorder tools/*.cm? tools/*.o
 	rm -f $(GENERATED) .depend
-	rm -f .lia.cache
 	$(MAKE) -f Makefile.extr clean
 	$(MAKE) -C runtime clean
 	$(MAKE) -C test clean
@@ -293,8 +290,12 @@ distclean:
 check-admitted: $(FILES)
 	@grep -w 'admit\|Admitted\|ADMITTED' $^ || echo "Nothing admitted."
 
+# Problems with coqchk (coq 8.6):
+# Integers.Int.Z_mod_modulus_range takes forever to check
+# compcert.backend.SelectDivproof.divs_mul_shift_2 takes forever to check
+
 check-proof: $(FILES)
-	$(COQCHK) compcert.driver.Complements
+	$(COQCHK) -admit compcert.lib.Integers -admit compcert.backend.SelectDivproof compcert.driver.Complements
 
 print-includes:
 	@echo $(COQINCLUDES)
